examples/pseudo_bool/cp_encoding/cp_to_ilp_newScript.sml
@@ -1,0 +1,1735 @@
+(*
+  Formalization of the CP to ILP phase
+*)
+open preamble cpTheory ilpTheory pbcTheory pbc_encodeTheory;
+
+val _ = new_theory "cp_to_ilp_new";
+
+(* The datatype for reified variables in the ILP encoding *)
+Datatype:
+  reif =
+  | Ge 'a int (* Reifies X ≥ i *)
+  | Eq 'a int (* Reifies X = i *)
+End
+
+(* The datatype for flags in the ILP encoding *)
+Datatype:
+  flag =
+  | Gt ('a + int) ('a + int)  (* Used to force in X ≠ Y *)
+  | Gem ('a + int) ('a + int) (* Used to force X ≥ Y in Array Max *)
+  | Eqc ('a + int) ('a + int) (* Used to force X = Y in Count *)
+  | Nv (('a + int) list) int (* Used to force some element in As = v *)
+  | Tb (('a + int) list) (('a + int) list) int
+End
+
+Definition reify_reif_def:
+  reify_reif wi eb ⇔
+  case eb of
+    Ge X i => wi X ≥ i
+  | Eq X i => wi X = i
+End
+
+Definition reify_flag_def:
+  reify_flag wi eb ⇔
+  case eb of
+    Gt X Y => varc wi X > varc wi Y
+End
+
+Definition reify_def:
+  reify wi e ⇔
+  case e of
+    INL eb => reify_reif wi eb
+  | INR (n,eb) => reify_flag wi eb
+End
+
+val eval_raw = LIST_CONJ
+  [iconstraint_sem_def,eval_ilin_term_def,iSUM_def,eval_lin_term_def];
+
+Definition min_iterm_def:
+  min_iterm bnd (c,X) =
+    let (lb,ub) = bnd X in
+      if c < 0i then c * ub
+      else c * lb
+End
+
+Theorem min_iterm_le:
+  valid_assignment bnd w ⇒
+  min_iterm bnd t ≤ eval_iterm w t
+Proof
+  Cases_on`t`>>
+  rw[valid_assignment_def,eval_iterm_def,min_iterm_def]>>
+  pairarg_tac>>gvs[]>>
+  first_x_assum drule>>gvs[]>>
+  rw[]
+  >- (
+    DEP_REWRITE_TAC[INT_LE_ANTIMONO]>>
+    simp[])
+  >>
+    match_mp_tac INT_LE_MONO_IMP>>
+    intLib.ARITH_TAC
+QED
+
+Definition min_ilin_term_def:
+  min_ilin_term bnd (xs:'a ilin_term) =
+  iSUM (MAP (min_iterm bnd) xs)
+End
+
+Theorem eval_ilin_term_min_ilin_term:
+  valid_assignment bnd w ⇒
+  min_ilin_term bnd xs ≤ eval_ilin_term w xs
+Proof
+  rw[min_ilin_term_def,eval_ilin_term_def]>>
+  match_mp_tac iSUM_MAP_le>>
+  rw[]>>
+  metis_tac[min_iterm_le]
+QED
+
+(* List of literals imply iconstraint under bounds *)
+Definition bits_imply_def:
+  bits_imply bnd xs cc =
+  case cc of (is,bs,c) =>
+    let r = c - min_ilin_term bnd is - min_lin_term bs in
+    let rr = int_max r 0 in
+    (is, MAP (λx. (rr, negate x)) xs ++ bs, c)
+End
+
+Theorem bits_imply_sem:
+  valid_assignment bnd wi ⇒
+  iconstraint_sem (bits_imply bnd xs c) (wi,wb) =
+    (EVERY (lit wb) xs ⇒ iconstraint_sem c (wi,wb))
+Proof
+  rw[bits_imply_def]>>
+  every_case_tac>>gvs[iconstraint_sem_def]>>
+  Cases_on`EVERY (lit wb) xs`
+  >- (
+    drule eval_lin_term_MAP_negate_0>> rw[])>>
+  simp[]>>
+  rename1`eval_ilin_term wi is + (_ + eval_lin_term wb bs) ≥ rr`>>
+  drule eval_ilin_term_min_ilin_term>>
+  disch_then(qspec_then`is` assume_tac)>>
+  `min_lin_term bs ≤ eval_lin_term wb bs` by
+    metis_tac[eval_lin_term_min_lin_term]>>
+  qmatch_goalsub_abbrev_tac`int_max r 0`>>
+  drule eval_lin_term_MAP_negate_ge>>
+  disch_then(qspec_then`int_max r 0` mp_tac)>>
+  impl_tac >- intLib.ARITH_TAC>>
+  rw[Abbr`r`]>>
+  intLib.ARITH_TAC
+QED
+
+Theorem eval_ilin_term_flip_coeffs[simp]:
+  eval_ilin_term w (flip_coeffs xs) = - eval_ilin_term w xs
+Proof
+  simp[eval_ilin_term_def,flip_coeffs_def]>>
+  Induct_on`xs`>>rw[iSUM_def]>>
+  pairarg_tac>>simp[]>>
+  intLib.ARITH_TAC
+QED
+
+Definition max_iterm_def:
+  max_iterm bnd (c,X) =
+    let (lb,ub) = bnd X in
+      if c < 0i then c * lb
+      else c * ub
+End
+
+Theorem max_iterm_le:
+  valid_assignment bnd w ⇒
+  eval_iterm w t ≤ max_iterm bnd t
+Proof
+  Cases_on`t`>>
+  rw[valid_assignment_def,eval_iterm_def,max_iterm_def]>>
+  pairarg_tac>>gvs[]>>rw[]>>
+  first_x_assum(qspec_then`r` mp_tac)>>gvs[]>>
+  rw[]
+  >- (
+    DEP_REWRITE_TAC[INT_LE_ANTIMONO]>>
+    simp[])
+  >>
+    match_mp_tac INT_LE_MONO_IMP>>
+    intLib.ARITH_TAC
+QED
+
+Definition max_ilin_term_def:
+  max_ilin_term bnd (xs:'a ilin_term) =
+  iSUM (MAP (max_iterm bnd) xs)
+End
+
+Theorem eval_ilin_term_max_ilin_term:
+  valid_assignment bnd w ⇒
+  eval_ilin_term w xs ≤ max_ilin_term bnd xs
+Proof
+  rw[max_ilin_term_def,eval_ilin_term_def]>>
+  match_mp_tac iSUM_MAP_le>>
+  rw[]>>
+  metis_tac[max_iterm_le]
+QED
+
+(* constraint implies list of literals *)
+Definition imply_bits_def:
+  imply_bits bnd xs cc =
+  case cc of (is,bs,c) =>
+    let nis = flip_coeffs is in
+    let nbs = flip_coeffs bs in
+    let nc = 1 - c in
+    let r = nc + max_ilin_term bnd is + max_lin_term bs in
+    let rr = int_max r 0 in
+    MAP (λx. (nis, (rr, x) :: nbs, nc)) xs
+End
+
+Theorem imply_bits_sem:
+  valid_assignment bnd wi ⇒
+  EVERY (λx. iconstraint_sem x (wi,wb)) (imply_bits bnd xs c)
+  =
+  (iconstraint_sem c (wi,wb) ⇒ EVERY (lit wb) xs)
+Proof
+  rw[imply_bits_def]>>
+  every_case_tac>>
+  gvs[EVERY_MEM,MEM_MAP,PULL_EXISTS,PULL_FORALL,iconstraint_sem_def]>>
+  ho_match_mp_tac
+    (METIS_PROVE []
+    ``
+      (∀x. (P x ⇒ (Q x ⇔ (A x ⇒ R x)))) ⇒
+      ((!x. (P x ⇒ Q x)) ⇔ (!x. (A x ⇒ P x ⇒ R x)))``)>>
+  rw[]>>
+  rename1`lit wb x`>>
+  Cases_on`lit wb x`>>simp[]
+  >- (
+    rename1`-eval_ilin_term wi is + (_ + -eval_lin_term wb bs) ≥ 1 - rr`>>
+    drule eval_ilin_term_max_ilin_term>>
+    disch_then(qspec_then`is` assume_tac)>>
+    `eval_lin_term wb bs ≤ max_lin_term bs` by
+      metis_tac[eval_lin_term_max_lin_term]>>
+    intLib.ARITH_TAC)>>
+  intLib.ARITH_TAC
+QED
+
+(* encodes iff *)
+Definition bimply_bits_def:
+  bimply_bits bnd xs cc =
+  bits_imply bnd xs cc ::
+  imply_bits bnd xs cc
+End
+
+Theorem bimply_bits_sem:
+  valid_assignment bnd wi ⇒
+  EVERY (λx. iconstraint_sem x (wi,wb)) (bimply_bits bnd xs c)
+  =
+  (iconstraint_sem c (wi,wb) ⇔ EVERY (lit wb) xs)
+Proof
+  rw[bimply_bits_def]>>
+  metis_tac[imply_bits_sem,bits_imply_sem]
+QED
+
+(* Encoding a single variable X_{>=i} ⇔ X ≥ i *)
+Definition encode_ge_def:
+  encode_ge bnd X i =
+  bimply_bits bnd [Pos (INL (Ge X i))] ([(1,X)],[],i)
+End
+
+Theorem encode_ge_sem:
+  valid_assignment bnd wi ⇒
+  EVERY (λx. iconstraint_sem x (wi,wb)) (encode_ge bnd X i)
+  =
+  (wb (INL (Ge X i)) ⇔ wi X ≥ i)
+Proof
+  rw[encode_ge_def]>>
+  simp[bimply_bits_sem,eval_raw]>>
+  metis_tac[]
+QED
+
+(* Encoding a single variable X = i
+  X_{=i} ⇔ X_{>=i} ∧ ~X_{>=i+1}
+*)
+Definition encode_eq_def:
+  encode_eq bnd X i =
+  bimply_bits bnd [Pos (INL (Eq X i))]
+    ([],[(1,Pos(INL (Ge X i)));(1, Neg (INL (Ge X (i+1))))],2)
+End
+
+Theorem encode_eq_sem:
+  valid_assignment bnd wi ∧
+  (wb (INL (Ge X i)) ⇔ wi X ≥ i) ∧
+  (wb (INL (Ge X (i+1))) ⇔ wi X ≥ i+1)
+  ⇒
+  EVERY (λx. iconstraint_sem x (wi,wb)) (encode_eq bnd X i)
+  =
+  (wb (INL (Eq X i)) ⇔ wi X = i)
+Proof
+  rw[encode_eq_def]>>
+  gs[bimply_bits_sem,eval_raw,b2i_alt]>>
+  rw[]>>
+  eq_tac>>rw[]>>
+  intLib.ARITH_TAC
+QED
+
+(* Encodes a * X + b * Y ≥ c where both terms are varc *)
+Definition mk_constraint_ge_def:
+  mk_constraint_ge (a:int) X (b:int) Y (c:int) =
+  case (X,Y) of
+    (INL vX, INL vY) =>
+      ([(a,vX);(b,vY)],[],c)
+  | (INL vX, INR cY) =>
+      ([(a,vX)],[],c - b * cY)
+  | (INR cX, INL vY) =>
+      ([(b,vY)],[],c - a * cX)
+  | (INR cX, INR cY) =>
+      ([],[],c - a * cX - b * cY)
+End
+
+Theorem mk_constraint_ge_sem:
+  iconstraint_sem (mk_constraint_ge a X b Y c) (wi,wb) ⇔
+  a * (varc wi X) + b * (varc wi Y) ≥ c
+Proof
+  rw[mk_constraint_ge_def]>>every_case_tac>>
+  gvs[varc_def,eval_raw]>>
+  intLib.ARITH_TAC
+QED
+
+Definition forget_b_ilp_def:
+  forget_b_ilp
+    ((is,bs,c):
+      ('a, 'a reif + (num # 'a flag)) iconstraint ) =
+    (is,MAP (λ(a,b). (a, map_lit (SUM_MAP I FST) b)) bs, c):
+      ('a, 'a reif + num) iconstraint
+End
+
+Definition forget_b_ilps_def[simp]:
+  forget_b_ilps ilps = MAP forget_b_ilp ilps
+End
+
+Definition vars_b_ilp_def:
+  vars_b_ilp (is,bs,c) =
+    set (MAP (lit_var o SND) bs)
+End
+
+Definition vars_b_ilps_def[simp]:
+  vars_b_ilps ilps =
+  BIGUNION (IMAGE vars_b_ilp (set ilps))
+End
+
+Definition inj_vars_b_ilps_def:
+  inj_vars_b_ilps (ilps : ('a, 'a reif + (num # 'a flag)) iconstraint list) ⇔
+  ∀i l l'.
+    INR (i,l) ∈ vars_b_ilps ilps ∧
+    INR (i,l') ∈ vars_b_ilps ilps ⇒
+    l = l'
+End
+
+Definition bound_vars_b_ilps_def:
+  bound_vars_b_ilps n n' ilps ⇔
+  n ≤ n' ∧
+  ∀i l.
+    INR (i,l) ∈ vars_b_ilps ilps ⇒
+    (n:num) ≤ i ∧ i < n'
+End
+
+Definition good_b_ilps_def:
+  good_b_ilps n n' ilps ⇔
+  bound_vars_b_ilps n n' ilps ∧
+  inj_vars_b_ilps ilps
+End
+
+Theorem good_b_ilps_emp[simp]:
+  good_b_ilps n n []
+Proof
+  rw[good_b_ilps_def,inj_vars_b_ilps_def,bound_vars_b_ilps_def]
+QED
+
+Theorem forget_b_ilps_inj_vars_b_ilps_1:
+  inj_vars_b_ilps ilps ∧
+  (∀i l l'.
+    wb (INR (i,l)) = wb (INR (i,l'))) ⇒
+  EVERY (λx. iconstraint_sem x (wi,wb)) ilps ⇒
+  EVERY (λx. iconstraint_sem x (wi,
+      (wb o SUM_MAP I (λb. (b, ARB))))) (forget_b_ilps ilps)
+Proof
+  cheat
+QED
+
+Theorem forget_b_ilps_inj_vars_b_ilps_2:
+  inj_vars_b_ilps ilps ∧
+  EVERY (λx. iconstraint_sem x (wi,wb)) (forget_b_ilps ilps) ⇒
+  EVERY (λx. iconstraint_sem x (wi, wb o SUM_MAP I FST)) ilps
+Proof
+  cheat
+QED
+
+Definition select_wb_def:
+  select_wb (wb:('a reif + (num # 'a flag) -> bool))
+    ilps =
+    (let vs = vars_b_ilps ilps in
+    wb o SUM_MAP I (λ(i,l). (i, @l. INR (i,l) ∈ vs))) :
+      ('a reif + (num # 'a flag) -> bool)
+End
+
+Theorem inj_vars_b_ilps_fix:
+  inj_vars_b_ilps ilps ∧
+  EVERY (λx. iconstraint_sem x (wi,wb)) ilps ⇒
+  EVERY (λx. iconstraint_sem x (wi,
+    select_wb wb ilps)) ilps
+Proof
+  cheat
+QED
+
+Theorem bound_vars_b_ilps_append:
+  bound_vars_b_ilps n1 n1' ilps1 ∧
+  bound_vars_b_ilps n2 n2' ilps2 ∧
+  n1' ≤ n2 ⇒
+  bound_vars_b_ilps n1 n2' (ilps1 ++ ilps2)
+Proof
+  rw[]>>
+  fs[bound_vars_b_ilps_def,PULL_EXISTS]>>rw[]>>
+  rpt(first_x_assum drule>>fs[])
+QED
+
+Theorem good_b_ilps_append:
+  good_b_ilps n1 n1' ilps1 ∧
+  good_b_ilps n2 n2' ilps2 ∧
+  n1' ≤ n2 ⇒
+  good_b_ilps n1 n2' (ilps1 ++ ilps2)
+Proof
+  rw[good_b_ilps_def]
+  >- metis_tac[bound_vars_b_ilps_append]>>
+  fs[inj_vars_b_ilps_def,PULL_EXISTS]>>rw[]
+  >- metis_tac[]
+  >- (
+    fs[bound_vars_b_ilps_def,PULL_EXISTS]>>
+    rpt (first_x_assum drule_all)>>
+    simp[])
+  >- (
+    fs[bound_vars_b_ilps_def,PULL_EXISTS]>>
+    rpt (first_x_assum drule_all)>>
+    simp[])
+  >- metis_tac[]
+QED
+
+Theorem map_lit_negate:
+  map_lit f (negate l) =
+  negate (map_lit f l)
+Proof
+  Cases_on`l`>>rw[negate_def,map_lit_def]
+QED
+
+Theorem min_lin_term_MAP_map_lit[simp]:
+  min_lin_term
+    (MAP (λ(a,b). (a,map_lit f b)) cc1) =
+  min_lin_term cc1
+Proof
+  rw[min_lin_term_def,MAP_MAP_o,o_DEF,LAMBDA_PROD]
+QED
+
+Theorem forget_b_ilp_bits_imply[simp]:
+  forget_b_ilp (bits_imply bnd xs cc) =
+  bits_imply bnd (MAP (map_lit (SUM_MAP I FST)) xs)
+    (forget_b_ilp cc)
+Proof
+  PairCases_on`cc`>>
+  rw[bits_imply_def,forget_b_ilp_def]>>
+  simp[MAP_MAP_o,o_DEF,map_lit_negate]
+QED
+
+Theorem forget_b_ilp_mk_constraint_ge[simp]:
+  forget_b_ilp (mk_constraint_ge a X b Y c) =
+  mk_constraint_ge a X b Y c
+Proof
+  rw[mk_constraint_ge_def]>>
+  every_case_tac>>fs[forget_b_ilp_def]
+QED
+
+Definition mk_fresh_def:
+  mk_fresh (n:num) rhs =
+    (n+1, INR (n, rhs:'a flag))
+End
+
+Theorem PAIR_MAP_o[simp]:
+  (f1 ## g1) ((f2 ## g2) p) =
+  (f1 o f2 ## g1 o g2) p
+Proof
+  rw[PAIR_MAP]
+QED
+
+Theorem lit_var_negate[simp]:
+  lit_var (negate x) = lit_var x
+Proof
+  Cases_on`x`>>rw[]
+QED
+
+Theorem vars_b_ilp_bits_imply[simp]:
+  vars_b_ilp (bits_imply bnd xs cc) =
+  set (MAP lit_var xs) ∪ vars_b_ilp cc
+Proof
+  PairCases_on`cc`>>
+  rw[bits_imply_def,vars_b_ilp_def,MAP_MAP_o,o_DEF,SF ETA_ss]
+QED
+
+Theorem vars_b_ilp_mk_constraint_ge[simp]:
+  vars_b_ilp (mk_constraint_ge a X b Y c) = {}
+Proof
+  rw[mk_constraint_ge_def]>>
+  every_case_tac>>fs[vars_b_ilp_def]
+QED
+
+(*** not_equals ***)
+Definition encode_not_equals_def:
+  encode_not_equals bnd n X Y =
+  (I ##
+    (λv.
+    [
+    bits_imply bnd [Pos v] (mk_constraint_ge 1 X (-1) Y 1);
+    bits_imply bnd [Neg v] (mk_constraint_ge 1 Y (-1) X 1)
+    ]))
+  (mk_fresh n (Gt X Y))
+End
+
+Definition cencode_not_equals_def:
+  cencode_not_equals bnd n X Y =
+  (I ## forget_b_ilps) (encode_not_equals bnd n X Y)
+End
+
+Theorem cencode_not_equals_compute =
+  SRULE [encode_not_equals_def,mk_fresh_def] cencode_not_equals_def;
+
+Theorem encode_not_equals_sem_1:
+  valid_assignment bnd wi ∧
+  not_equals_sem X Y wi ⇒
+  EVERY (λx. iconstraint_sem x (wi,reify wi))
+    (SND (encode_not_equals bnd n X Y))
+Proof
+  rw[mk_fresh_def,not_equals_sem_def,encode_not_equals_def,bits_imply_sem,mk_constraint_ge_sem,reify_def,reify_flag_def]>>
+  intLib.ARITH_TAC
+QED
+
+Theorem encode_not_equals_sem_2:
+  valid_assignment bnd wi ∧
+  EVERY (λx. iconstraint_sem x (wi,wb))
+    (SND (encode_not_equals bnd n X Y)) ⇒
+  not_equals_sem X Y wi
+Proof
+  rw[encode_not_equals_def,not_equals_sem_def]>>
+  rfs[bits_imply_sem,mk_constraint_ge_sem]>>
+  rename1`wb f`>>
+  Cases_on`wb f` >> fs[]>>
+  intLib.ARITH_TAC
+QED
+
+Theorem encode_not_equals_good_b_ilps:
+  encode_not_equals bnd n X Y = (n', ilps) ⇒
+  good_b_ilps n n' ilps
+Proof
+  rw[encode_not_equals_def]>>
+  simp[good_b_ilps_def,inj_vars_b_ilps_def,bound_vars_b_ilps_def,vars_b_ilps_def]>>
+  gvs[mk_fresh_def]
+QED
+
+(*** all_different ***)
+
+(* Step 0: define the abstract encoding *)
+Definition encode_all_different_row_def:
+  (encode_all_different_row bnd n A [] = (n,[])) ∧
+  (encode_all_different_row bnd n A (B::Bs) =
+    let (n',B') = encode_not_equals bnd n A B in
+    let (n'',Bs') = encode_all_different_row bnd n' A Bs in
+      (n'',B' ++ Bs'))
+End
+
+Definition encode_all_different_def:
+  (encode_all_different bnd n [] = (n,[])) ∧
+  (encode_all_different bnd n (A::As) =
+    let (n',A') = encode_all_different_row bnd n A As in
+    let (n'',As') = encode_all_different bnd n' As in
+    (n'',A' ++ As'))
+End
+
+Definition all_different_row_sem_def:
+  all_different_row_sem w A As ⇔
+   ¬ MEM (varc w A) (MAP (varc w) As)
+End
+
+(* Step 1: prove the sem_1 and sem_2 theorems *)
+Theorem encode_all_different_row_sem_1:
+  valid_assignment bnd wi ∧
+  all_different_row_sem wi A As ⇒
+  EVERY (λx. iconstraint_sem x (wi,reify wi))
+    (SND (encode_all_different_row bnd n A As))
+Proof
+  qid_spec_tac`n`>>
+  Induct_on`As`>>rw[encode_all_different_row_def]>>
+  fs[all_different_row_sem_def]>>
+  pairarg_tac>>gvs[]>>
+  pairarg_tac>>gvs[]>>
+  metis_tac[encode_not_equals_sem_1,SND,not_equals_sem_def]
+QED
+
+Theorem encode_all_different_row_sem_2:
+  valid_assignment bnd wi ∧
+  EVERY (λx. iconstraint_sem x (wi,wb))
+    (SND (encode_all_different_row bnd n A As)) ⇒
+  all_different_row_sem wi A As
+Proof
+  qid_spec_tac`n`>>
+  Induct_on`As`>>rw[encode_all_different_row_def]>>
+  fs[all_different_row_sem_def]>>
+  pairarg_tac>>gvs[]>>
+  pairarg_tac>>gvs[]>>
+  metis_tac[encode_not_equals_sem_2,SND,not_equals_sem_def]
+QED
+
+Theorem encode_all_different_sem_1:
+  valid_assignment bnd wi ∧
+  all_different_sem As wi ⇒
+  EVERY (λx. iconstraint_sem x (wi,reify wi))
+    (SND (encode_all_different bnd n As))
+Proof
+  qid_spec_tac`n`>>
+  Induct_on`As`>>rw[encode_all_different_def]>>
+  fs[all_different_sem_def]>>
+  pairarg_tac>>gvs[]>>
+  pairarg_tac>>gvs[]>>
+  metis_tac[encode_all_different_row_sem_1,SND,all_different_row_sem_def]
+QED
+
+Theorem encode_all_different_sem_2:
+  valid_assignment bnd wi ∧
+  EVERY (λx. iconstraint_sem x (wi,wb))
+    (SND (encode_all_different bnd n As)) ⇒
+  all_different_sem As wi
+Proof
+  qid_spec_tac`n`>>
+  Induct_on`As`>>rw[encode_all_different_def]>>
+  fs[all_different_sem_def]>>
+  pairarg_tac>>gvs[]>>
+  pairarg_tac>>gvs[]>>
+  metis_tac[encode_all_different_row_sem_2,SND,all_different_row_sem_def]
+QED
+
+(* Step 2: define the cencode and prove it correct *)
+Definition cencode_all_different_row_def:
+  (cencode_all_different_row bnd n A [] = (n,[])) ∧
+  (cencode_all_different_row bnd n A (B::Bs) =
+    let (n',B') = cencode_not_equals bnd n A B in
+    let (n'',Bs') = cencode_all_different_row bnd n' A Bs in
+      (n'',B' ++ Bs'))
+End
+
+Definition cencode_all_different_def:
+  (cencode_all_different bnd n [] = (n,[])) ∧
+  (cencode_all_different bnd n (A::As) =
+    let (n',A') = cencode_all_different_row bnd n A As in
+    let (n'',As') = cencode_all_different bnd n' As in
+    (n'',A' ++ As'))
+End
+
+Theorem cencode_all_different_row_forget_ilps:
+  cencode_all_different_row bnd n A As =
+  (I ## forget_b_ilps)
+    (encode_all_different_row bnd n A As)
+Proof
+  qid_spec_tac`n`>>Induct_on`As`>>
+  rw[cencode_all_different_row_def,encode_all_different_row_def,cencode_not_equals_def]>>
+  pairarg_tac>>gvs[]>>
+  pairarg_tac>>gvs[]
+QED
+
+Theorem cencode_all_different_forget_ilps:
+  cencode_all_different bnd n As =
+  (I ## forget_b_ilps)
+    (encode_all_different bnd n As)
+Proof
+  qid_spec_tac`n`>>Induct_on`As`>>
+  rw[cencode_all_different_def,encode_all_different_def,cencode_all_different_row_forget_ilps]>>
+  pairarg_tac>>gvs[]>>
+  pairarg_tac>>gvs[]
+QED
+
+(* Step 3: bound_vars and inj_vars properties *)
+Theorem encode_all_different_row_good_b_ilps:
+  encode_all_different_row bnd n A As = (n', ilps) ⇒
+  good_b_ilps n n' ilps
+Proof
+  qid_spec_tac`n`>>qid_spec_tac`ilps`>>
+  Induct_on`As`>>
+  rw[encode_all_different_row_def]>>
+  rpt (pairarg_tac>>gvs[])>>
+  irule_at Any good_b_ilps_append>>
+  drule encode_not_equals_good_b_ilps>>
+  disch_then (irule_at Any)>>
+  first_x_assum drule>>
+  disch_then (irule_at Any)>>
+  simp[]
+QED
+
+Theorem encode_all_different_good_b_ilps:
+  encode_all_different bnd n As = (n', ilps) ⇒
+  good_b_ilps n n' ilps
+Proof
+  qid_spec_tac`n`>>qid_spec_tac`ilps`>>
+  Induct_on`As`>>
+  rw[encode_all_different_def]>>
+  rpt (pairarg_tac>>gvs[])>>
+  irule_at Any good_b_ilps_append>>
+  drule encode_all_different_row_good_b_ilps>>
+  disch_then (irule_at Any)>>
+  first_x_assum drule>>
+  disch_then (irule_at Any)>>
+  simp[]
+QED
+
+(*** abs ***)
+
+(* Only uses reifications *)
+
+(* Encoding for Y a variable *)
+Definition encode_abs_var_def:
+  encode_abs_var bnd X Y =
+  let vY = INL Y in
+  encode_ge bnd Y 0 ++
+  [
+    bits_imply bnd [Pos (INL (Ge Y 0))] (mk_constraint_ge 1 X (-1) vY 0);
+    bits_imply bnd [Pos (INL (Ge Y 0))] (mk_constraint_ge 1 vY (-1) X 0);
+    bits_imply bnd [Neg (INL (Ge Y 0))] (mk_constraint_ge 1 X 1 vY 0);
+    bits_imply bnd [Neg (INL (Ge Y 0))] (mk_constraint_ge (-1) X (-1) vY 0);
+  ]
+End
+
+Theorem encode_abs_var_sem:
+  valid_assignment bnd wi
+  ⇒
+  EVERY (λx. iconstraint_sem x (wi,wb)) (encode_abs_var bnd X Y)
+  =
+  (
+    (wb (INL (Ge Y 0)) ⇔ wi Y ≥ 0) ∧
+    abs_sem X (INL Y) wi
+  )
+Proof
+  rw[encode_abs_var_def]>>
+  match_mp_tac LEFT_AND_CONG>>
+  CONJ_TAC >- simp[encode_ge_sem]>>
+  strip_tac>>
+  simp[bits_imply_sem,mk_constraint_ge_sem,abs_sem_def]>>
+  `varc wi (INL Y) = wi Y` by simp[varc_def]>>
+  intLib.ARITH_TAC
+QED
+
+Definition encode_abs_const_def:
+  encode_abs_const X Y =
+  if Y ≥ 0 then
+  [
+    mk_constraint_ge 1 X (-1) (INR Y) 0;
+    mk_constraint_ge (-1) X 1 (INR Y) 0;
+  ]
+  else
+  [
+    mk_constraint_ge 1 X 1 (INR Y) 0;
+    mk_constraint_ge (-1) X (-1) (INR Y) 0;
+  ]
+End
+
+Theorem encode_abs_const_sem:
+  EVERY (λx. iconstraint_sem x (wi,wb)) (encode_abs_const X Y)
+  =
+  abs_sem X (INR Y) wi
+Proof
+  rw[encode_abs_const_def]>>
+  simp[abs_sem_def,mk_constraint_ge_sem]>>
+  `varc wi (INR Y) = Y` by simp[varc_def]>>
+  simp[]>>
+  intLib.ARITH_TAC
+QED
+
+Definition encode_abs_def:
+  encode_abs bnd X Y =
+  case Y of
+    INL vY => encode_abs_var bnd X vY
+  | INR cY => encode_abs_const X cY
+End
+
+(* TODO: not updated below here *)
+Theorem encode_abs_sem:
+  valid_assignment bnd wi
+  ⇒
+  EVERY (λx. iconstraint_sem x (wi,wb)) (encode_abs bnd X Y)
+  =
+  (
+  (case Y of INR _ => T | INL Y =>
+  (wb (Ge Y 0) ⇔ wi Y ≥ 0)) ∧
+  abs_sem X Y wi)
+Proof
+  rw[encode_abs_def]>>
+  TOP_CASE_TAC>>gvs[]
+  >-
+    metis_tac[encode_abs_var_sem]
+  >>
+    metis_tac[encode_abs_const_sem]
+QED
+
+
+Definition encode_cp_one_def:
+  encode_cp_one bnd c =
+  case c of
+    NotEquals X Y => encode_not_equals bnd X Y
+  | AllDifferent As => encode_all_different bnd As
+  | Element R X As => encode_element bnd R X As
+  | Abs X Y => encode_abs bnd X Y
+  | Ilc Xs op rhs => encode_ilc Xs op rhs
+End
+
+Theorem encode_cp_one_sem_1:
+  valid_assignment bnd wi ∧
+  constraint_sem c wi ⇒
+  EVERY (λx. iconstraint_sem x (wi,reify_reif wi)) (encode_cp_one bnd c)
+Proof
+  Cases_on`c`>>
+  rw[encode_cp_one_def,constraint_sem_def]
+  >- (
+    simp[encode_not_equals_sem,reify_reif_def]>>
+    gvs[not_equals_sem_def]>>
+    intLib.ARITH_TAC)
+  >- (
+    simp[encode_all_different_sem,reify_reif_def]>>
+    gvs[all_different_sem_def,EL_ALL_DISTINCT_EL_EQ]>>
+    rw[]>>
+    first_x_assum(qspecl_then[`i`,`j`] mp_tac)>>
+    simp[EL_MAP]>>
+    intLib.ARITH_TAC)
+  >- (
+    simp[encode_element_sem,reify_reif_def]>>
+    every_case_tac>>simp[])
+  >- (
+    simp[encode_abs_sem,reify_reif_def]>>
+    every_case_tac>>simp[])
+  >- (
+    simp[encode_ilc_sem,reify_reif_def]>>
+    every_case_tac>>simp[])
+QED
+
+Theorem encode_cp_one_sem_2:
+  valid_assignment bnd wi ∧
+  EVERY (λx. iconstraint_sem x (wi,wb)) (encode_cp_one bnd c) ⇒
+  constraint_sem c wi
+Proof
+  Cases_on`c`>>
+  rw[encode_cp_one_def,constraint_sem_def]
+  >-
+    gvs[encode_not_equals_sem]
+  >-
+    gvs[encode_all_different_sem]
+  >-
+    gvs[encode_element_sem]
+  >-
+    gvs[encode_abs_sem]
+  >-
+    gvs[encode_ilc_sem]
+QED
+
+(* An actual implementation will avoid duplicates here *)
+Definition encode_cp_all_def:
+  encode_cp_all bnd cs =
+  FLAT (MAP (encode_cp_one bnd) cs)
+End
+
+Theorem encode_cp_all_sem_1:
+  valid_assignment bnd wi ∧
+  EVERY (λc. constraint_sem c wi) cs ⇒
+  EVERY (λx. iconstraint_sem x (wi,reify_reif wi)) (encode_cp_all bnd cs)
+Proof
+  simp[encode_cp_all_def,EVERY_FLAT]>>
+  simp[Once EVERY_MEM]>>
+  rw[Once EVERY_MEM,MEM_MAP]>>
+  metis_tac[encode_cp_one_sem_1]
+QED
+
+Theorem encode_cp_all_sem_2:
+  valid_assignment bnd wi ∧
+  EVERY (λx. iconstraint_sem x (wi,wb)) (encode_cp_all bnd cs) ⇒
+  EVERY (λc. constraint_sem c wi) cs
+Proof
+  simp[encode_cp_all_def,EVERY_FLAT]>>
+  rw[Once EVERY_MEM,MEM_MAP,PULL_EXISTS]>>
+  simp[Once EVERY_MEM]>>
+  metis_tac[encode_cp_one_sem_2]
+QED
+
+(* === Examples ===
+
+not-equals
+  EVAL``encode_not_equals (λX. (-10,10)) (INL X) (INL Y)``
+  EVAL``encode_not_equals (λX. (-10,10)) (INL X) (INR 4)``
+
+all-different
+  EVAL``encode_all_different (λX. (-10,10)) [INL X; INL Y; INL Z; INR 0i]``
+
+element
+  EVAL``encode_element (λX. (-10,10)) (INL R) (INL X) [INL A; INL B; INL C; INL D; INL E]``
+
+abs
+  EVAL``encode_abs (λX. (-10,10)) (INL X) (INL Y)``
+
+*)
+
+
+
+Definition augment_assignment_def:
+  augment_assignment wb wc b =
+    case b of
+      INL b => wb b
+    | INR c => wc c
+End
+
+Definition augment_iassignment_def:
+  augment_iassignment (wi,wb) wc =
+  (wi, augment_assignment wb wc)
+End
+
+Definition exists_sem_def:
+  exists_sem (ls : ('a,('b + 'c)) iconstraint list)
+    (w :('a,'b) iassignment) ⇔
+  ∃wc: ('c -> bool).
+    EVERY (λc. iconstraint_sem c
+    (augment_iassignment w wc)) ls
+End
+
+Theorem encode_not_equals_sem:
+  valid_assignment bnd wi ⇒
+  (not_equals_sem X Y wi ⇔
+   exists_sem
+     (encode_not_equals bnd n X Y) (wi,wb))
+Proof
+  strip_tac>>
+  simp[exists_sem_def,not_equals_sem_def]>>
+  simp[encode_not_equals_def,bits_imply_sem,mk_constraint_ge_sem,augment_iassignment_def,augment_assignment_def]>>
+  eq_tac>>rw[]
+  >- (
+    qexists_tac`λb. varc wi X > varc wi Y`>>
+    simp[]>>
+    intLib.ARITH_TAC)>>
+  Cases_on`wc (Ne n X Y)`>>fs[]>>
+  intLib.ARITH_TAC
+QED
+
+(* Forgets a named variable *)
+Definition forget_var_def:
+  forget_var (ln,n:num) v =
+  case FLOOKUP ln v of
+    SOME m => (m, (ln,n))
+  | NONE =>
+    (n, (ln |+ (v,n),n+1))
+End
+
+(* Forgets a literal name on the right *)
+Definition forget_lit_def:
+  forget_lit lnn l =
+  case l of
+    Pos (INR v) =>
+    let (n,lnn') = forget_var lnn v in
+      (Pos (INR n), lnn')
+  | Neg (INR v) =>
+    let (n,lnn') = forget_var lnn v in
+      (Neg (INR n), lnn')
+  | Pos (INL v) => (Pos (INL v), lnn)
+  | Neg (INL v) => (Neg (INL v), lnn)
+End
+
+(* Forgets names in a lin term *)
+Definition forget_lin_term_def:
+  (forget_lin_term lnn [] =
+     ([],lnn)) ∧
+  (forget_lin_term lnn ((c,l)::ls) =
+    let (l',lnn') = forget_lit lnn l in
+    let (ls',lnn'') = forget_lin_term lnn' ls in
+    ((c,l')::ls', lnn''))
+End
+
+Definition forget_iconstraint_def:
+  forget_iconstraint lnn
+    ((is,bs,c) : ('a, 'a reif + 'a flag) iconstraint) =
+  let (bs',lnn') = forget_lin_term lnn bs in
+    ((is,bs',c),lnn')
+End
+
+(* Forget over an existentially quantified block *)
+Definition forget_exists_aux_def:
+  (forget_exists_aux lnn [] = ([],lnn)) ∧
+  (forget_exists_aux lnn (ic::ics) =
+    let (ic',lnn') = forget_iconstraint lnn ic in
+    let (ics',lnn'') = forget_exists_aux lnn' ics in
+    ((ic'::ics'),lnn''))
+End
+
+Definition forget_exists_def:
+  forget_exists n ics =
+    let (ics',lnn') = forget_exists_aux (FEMPTY,n) ics in
+    (ics',SND lnn')
+End
+
+Definition forget_all_aux_def:
+  (forget_all_aux n [] = []) ∧
+  (forget_all_aux n (ics::icss) =
+    let (ic',n') = forget_iconstraint lnn ic in
+      ic'::forget_all_aux
+    
+  [] = []) ∧
+  SND (FOLDL forget_exists (0n,[]) icss)
+End
+
+
+(* Forget the entire list of constraints *)
+Definition forget_all_def:
+  forget_all icss =
+  SND (FOLDL forget_exists (0n,[]) icss)
+End
+
+Definition exists_sem_def:
+  exists_sem (lss : ('a,('b + 'c)) iconstraint list list)
+    (w :('a,'b) iassignment) ⇔
+  EVERY
+    (λls.
+      ∃wc: ('c -> bool).
+        EVERY (λc. iconstraint_sem c
+          (augment_iassignment w wc)) ls) lss
+End
+
+
+
+Type iconstraint = ``:'a ilin_term # 'b lin_term # int``
+
+
+
+Definition fencode_not_equals_def:
+  fencode_not_equals bnd n X Y =
+  [
+    bits_imply bnd [Pos (Fresh n)] (mk_constraint_ge 1 X (-1) Y 1);
+    bits_imply bnd [Neg (Fresh n)] (mk_constraint_ge 1 Y (-1) X 1)
+  ]
+End
+
+Theorem foo:
+  forget (encode bnd n X Y)
+
+
+
+(* X_{=i} ⇒ Ai = R where Ai, R can be Varc *)
+Definition encode_element_eq_def:
+  encode_element_eq bnd R X (i:num,Ai) =
+  [
+    bits_imply bnd [Pos (Eq X (&(i+1)))] (mk_constraint_ge 1 Ai (-1) R 0);
+    bits_imply bnd [Pos (Eq X (&(i+1)))] (mk_constraint_ge 1 R (-1) Ai 0)
+  ]
+End
+
+Theorem encode_element_eq_sem:
+  valid_assignment bnd wi ∧
+  (wb (Eq X &(i+1)) ⇔ wi X = &(i+1))
+  ⇒
+  EVERY (λx. iconstraint_sem x (wi,wb)) (encode_element_eq bnd R X (i,Ai))
+  =
+  (wi X = &(i+1) ⇒ varc wi R = varc wi Ai)
+Proof
+  rw[encode_element_eq_def,eval_raw,bits_imply_sem,mk_constraint_ge_sem]>>
+  rw[]>>
+  intLib.ARITH_TAC
+QED
+
+(* Adds X ≥ 1, - X ≥ -|As| where needed *)
+Definition encode_element_var_def:
+  encode_element_var (bnd:'a bounds) R X As =
+  let (lb:int,ub:int) = bnd X in
+  let (len:int) = &(LENGTH As) in
+  let ges = FLAT (GENLIST (λi. encode_ge bnd X &(i+1)) (LENGTH As + 1)) in
+  let eqs = FLAT (GENLIST (λi. encode_eq bnd X &(i+1)) (LENGTH As)) in
+  let xlb = if lb < 1 then [([(1i,X)],[],1i)] else [] in
+  let xub = if len < ub then [([(-1i,X)],[],-len)] else [] in
+    ges ++ eqs ++ xlb ++ xub ++
+    FLAT (MAP (encode_element_eq bnd R X) (enumerate 0n As))
+End
+
+(* TODO: copied from npbc_check, move into misc... *)
+Theorem MEM_enumerate_index:
+  ∀k xs.
+  MEM (i,e) (enumerate k xs) ⇒
+  ∃j. j < LENGTH xs ∧ i = k + j
+Proof
+  Induct_on`xs`>>rw[miscTheory.enumerate_def]
+  >- intLib.ARITH_TAC>>
+  first_x_assum drule>>
+  rw[]
+  >- intLib.ARITH_TAC
+QED
+
+Theorem MEM_enumerate_iff:
+  MEM ie (enumerate 0 xs) ⇔
+  ∃i e. ie = (i,e) ∧ i < LENGTH xs ∧ EL i xs = e
+Proof
+  Cases_on`ie`>>
+  rename1`MEM (i,e) _ `>>
+  Cases_on`i < LENGTH xs`>>fs[MEM_enumerate]
+  >- metis_tac[]>>
+  CCONTR_TAC>>fs[]>>
+  drule MEM_enumerate_index>>
+  rw[]
+QED
+
+(* TODO: is this style better? *)
+Theorem encode_element_var_sem:
+  valid_assignment bnd wi
+  ⇒
+  EVERY (λx. iconstraint_sem x (wi,wb)) (encode_element_var bnd R X As)
+  =
+  (
+  (∀i. 1 ≤ i ∧ i ≤ LENGTH As + 1 ⇒
+    (wb (Ge X &i) ⇔ wi X ≥ &i)) ∧
+  (∀i. 1 ≤ i ∧ i ≤ LENGTH As ⇒
+    (wb (Eq X &i) ⇔ wi X = &i)) ∧
+  element_sem R (INL X) As wi)
+Proof
+  rw[encode_element_var_def]>>
+  pairarg_tac>>simp[element_sem_def]>>
+  simp[GSYM CONJ_ASSOC]>>
+  match_mp_tac LEFT_AND_CONG>>
+  CONJ_TAC >- (
+    simp[EVERY_FLAT,EVERY_GENLIST,encode_ge_sem]>>
+    eq_tac>>rw[]>>
+    first_x_assum(qspec_then`i-1` mp_tac)>>simp[])>>
+  strip_tac>>
+  match_mp_tac LEFT_AND_CONG>>
+  (* annoying ... *)
+  CONJ_TAC >- (
+    simp[EVERY_FLAT,EVERY_GENLIST]>>
+    eq_tac>>rw[]
+    >- (
+      DEP_REWRITE_TAC[GSYM encode_eq_sem]>>
+      simp[]>>
+      first_x_assum(qspec_then`i-1`mp_tac)>>
+      simp[]>>
+      first_x_assum(qspec_then`i + 1 `mp_tac)>>
+      simp[]>>
+      `&(i+1) = &i + 1i` by intLib.ARITH_TAC>>
+      simp[])>>
+    DEP_REWRITE_TAC[encode_eq_sem]>>
+    simp[]>>
+    last_x_assum(qspec_then`i + 1 + 1`mp_tac)>>
+      `&(i+2) = &(i + 1) + 1i` by intLib.ARITH_TAC>>
+    simp[])>>
+  strip_tac>>
+  match_mp_tac LEFT_AND_CONG>>
+  CONJ_TAC >- (
+    gvs[varc_def,valid_assignment_def]>>
+    first_x_assum drule>>rw[eval_raw]>>
+    intLib.ARITH_TAC)>>
+  strip_tac>>
+  match_mp_tac LEFT_AND_CONG>>
+  CONJ_TAC >- (
+    gvs[varc_def,valid_assignment_def]>>
+    first_x_assum drule>>rw[eval_raw]>>
+    intLib.ARITH_TAC)>>
+  strip_tac>>
+  rw[EVERY_FLAT,EVERY_MAP]>>
+  `∀x. MEM x (enumerate 0 As) ⇒
+       (EVERY (λx. iconstraint_sem x (wi,wb)) (encode_element_eq bnd R X x) ⇔
+       (wi X = &(FST x + 1) ⇒ varc wi R = varc wi (SND x)))` by (
+    Cases>>rw[]>>
+    match_mp_tac encode_element_eq_sem>>
+    simp[]>>
+    first_x_assum match_mp_tac>>
+    gvs[MEM_enumerate_iff])>>
+  `EVERY (λx.
+      EVERY (λx. iconstraint_sem x (wi,wb))
+      (encode_element_eq bnd R X x)) (enumerate 0 As) ⇔
+   EVERY (λx.
+      (wi X = &(FST x + 1) ⇒ varc wi R = varc wi (SND x))) (enumerate 0 As)` by
+   (match_mp_tac EVERY_CONG>>
+   simp[])>>
+  simp[EVERY_MEM,MEM_enumerate_iff,PULL_EXISTS] >>
+  eq_tac>>rw[]
+  >- (
+    first_x_assum irule>>
+    gvs[varc_def]>>
+    intLib.ARITH_TAC)>>
+  simp[varc_def]
+QED
+
+Definition encode_element_const_def:
+  encode_element_const R (X:int) As =
+  if 1 ≤ X ∧ X ≤ &(LENGTH As)
+  then
+    let Ai = EL (Num X -1) As in
+    [mk_constraint_ge 1 Ai (-1) R 0;
+     mk_constraint_ge 1 R (-1) Ai 0]
+  else
+    [([],[],1)]
+End
+
+Theorem encode_element_const_sem:
+  EVERY (λx. iconstraint_sem x (wi,wb)) (encode_element_const R X As)
+  =
+  element_sem R (INR X) As wi
+Proof
+  rw[encode_element_const_def,eval_raw,mk_constraint_ge_sem,element_sem_def]
+  >- (
+    simp[varc_def]>>
+    eq_tac>>rw[]>>
+    intLib.ARITH_TAC)>>
+  fs[varc_def]>>
+  intLib.ARITH_TAC
+QED
+
+Definition encode_element_def:
+  encode_element bnd R X As =
+  case X of
+    INL vX => encode_element_var bnd R vX As
+  | INR cX => encode_element_const R cX As
+End
+
+(* TODO: This seem too precise *)
+Theorem encode_element_sem:
+  valid_assignment bnd wi
+  ⇒
+  EVERY (λx. iconstraint_sem x (wi,wb)) (encode_element bnd R X As)
+  =
+  (
+  (case X of INR _ => T | INL X =>
+  (∀i. 1 ≤ i ∧ i ≤ LENGTH As + 1 ⇒
+    (wb (Ge X &i) ⇔ wi X ≥ &i)) ∧
+  (∀i. 1 ≤ i ∧ i ≤ LENGTH As ⇒
+    (wb (Eq X &i) ⇔ wi X = &i))) ∧
+  element_sem R X As wi)
+Proof
+  rw[encode_element_def]>>
+  TOP_CASE_TAC>>gvs[]
+  >-
+    metis_tac[encode_element_var_sem]
+  >>
+    metis_tac[encode_element_const_sem]
+QED
+
+Definition reify_reif_def:
+  reify_reif wi eb ⇔
+  case eb of
+    Ge X i => wi X ≥ i
+  | Eq X i => wi X = i
+  | Ne X Y => varc wi X > varc wi Y
+  | Gem X Y => varc wi X ≥ varc wi Y
+  | Eqc X Y => varc wi X = varc wi Y
+End
+
+Theorem encode_element_sem_1:
+  valid_assignment bnd wi ∧
+  element_sem R X As wi ⇒
+  EVERY (λx. iconstraint_sem x (wi,reify_reif wi)) (encode_element bnd R X As)
+Proof
+  rw[encode_element_def]>>
+  TOP_CASE_TAC>>gvs[]
+  >- (
+    DEP_REWRITE_TAC [encode_element_var_sem]>>
+    simp[reify_reif_def])
+  >>
+    metis_tac[encode_element_const_sem]
+QED
+
+Theorem encode_element_sem_2:
+  valid_assignment bnd wi ∧
+  EVERY (λx. iconstraint_sem x (wi,wb)) (encode_element bnd R X As) ⇒
+  element_sem R X As wi
+Proof
+  rw[encode_element_def]>>
+  every_case_tac>>gvs[]
+  >- (
+    pop_assum mp_tac>>
+    DEP_REWRITE_TAC[encode_element_var_sem]>>
+    simp[])
+  >>
+    metis_tac[encode_element_const_sem]
+QED
+
+Theorem all_different_sem_aux:
+  (∀i j. i < j ∧ j < LENGTH As ⇒
+    let X = EL i As in
+    let Y = EL j As in
+    if wb (Ne X Y)
+    then varc wi X > varc wi Y
+    else varc wi Y > varc wi X) ⇒
+  all_different_sem As wi
+Proof
+  rw[all_different_sem_def,EL_ALL_DISTINCT_EL_EQ]>>
+  Cases_on`n1 = n2`>>simp[]>>
+  wlog_tac `n1 < n2` [`n1`,`n2`]
+  >- (
+    `n2 < n1` by fs[]>>
+    first_x_assum drule_all>>
+    simp[])>>
+  first_x_assum drule>>
+  rw[EL_MAP]>>
+  intLib.ARITH_TAC
+QED
+
+Theorem encode_all_different_sem:
+  valid_assignment bnd wi ⇒
+  EVERY (λx. iconstraint_sem x (wi,wb)) (encode_all_different bnd As)
+  =
+  (
+  (∀i j. i < j ∧ j < LENGTH As ⇒
+    let X = EL i As in
+    let Y = EL j As in
+    if wb (Ne X Y)
+    then varc wi X > varc wi Y
+    else varc wi Y > varc wi X) ∧
+  all_different_sem As wi)
+Proof
+  simp[MATCH_MP IMP_AND_LEFT all_different_sem_aux]>>
+  rw[encode_all_different_def, EVERY_FLAT, EVERY_GENLIST]>>
+  eq_tac>>rw[]>>
+  gvs[PULL_FORALL]
+  >- (
+    first_x_assum(qspecl_then[`i`,`j`] mp_tac)>>
+    simp[encode_not_equals_sem])>>
+  rw[]>>
+  first_x_assum drule_all>>
+  metis_tac[encode_not_equals_sem,not_equals_sem_aux]
+QED
+
+Definition split_iclin_term_def:
+  (split_iclin_term ([]:'a iclin_term)
+    (acc:'a ilin_term) rhs = (acc,rhs)) ∧
+  (split_iclin_term ((c,X)::xs) acc rhs =
+    case X of
+      INL v => split_iclin_term xs ((c,v)::acc) rhs
+    | INR cc =>
+      split_iclin_term xs acc (rhs - c * cc))
+End
+
+Theorem split_iclin_term_sound:
+  ∀Xs rhs acc xs rhs'.
+    split_iclin_term Xs acc rhs = (xs,rhs') ⇒
+    eval_iclin_term wi Xs + eval_ilin_term wi acc - rhs =
+    eval_ilin_term wi xs - rhs'
+Proof
+  Induct
+  >-simp[split_iclin_term_def, eval_iclin_term_def, eval_ilin_term_def, iSUM_def]
+  >-(
+    Cases>>
+    Cases_on ‘r’>>
+    rw[split_iclin_term_def]>>
+    last_x_assum $ drule_then mp_tac>>
+    rw[eval_iclin_term_def, eval_ilin_term_def, iSUM_def, varc_def]>>
+    intLib.ARITH_TAC)
+QED
+
+Definition encode_ilc_def:
+  encode_ilc (Xs:'a iclin_term) (op:pbop) (rhs:int) =
+  let (xs,rhs) = split_iclin_term Xs [] rhs in
+  case op of
+    GreaterEqual => [(xs, [], rhs)]
+  | Greater => [(xs, [] , rhs+1)]
+  | LessEqual => [(MAP (λ(x:int, y). (-x, y)) xs, [], -rhs)]
+  | Less => [(MAP (λ(x:int, y). (-x, y)) xs, [], -rhs+1)]
+  | Equal => [(xs, [], rhs); (MAP (λ(x:int, y). (-x, y)) xs, [], -rhs)]
+End
+
+Theorem encode_ilc_sem:
+  EVERY (λx. iconstraint_sem x (wi,wb)) (encode_ilc Xs op rhs)
+  ⇔
+  ilc_sem Xs op rhs wi
+Proof
+  rw[encode_ilc_def,ilc_sem_def]>>
+  pairarg_tac>>gvs[]>>
+  CASE_TAC>>
+  simp[iconstraint_sem_def, eval_lin_term_def, iSUM_def]>>
+  ‘∀xs. eval_ilin_term wi (MAP (λ(x,y). (-x,y)) xs) = -(eval_ilin_term wi xs)’ by (
+    Induct
+    >-simp[eval_ilin_term_def, iSUM_def]
+    >-(
+      Cases>>
+      pop_assum mp_tac>>
+      simp[eval_ilin_term_def, iSUM_def]>>
+      intLib.ARITH_TAC))>>
+  pop_assum (fn thm => simp[thm])>>
+  drule_then (qspec_then ‘wi’ mp_tac) split_iclin_term_sound>>
+  rw[Once eval_ilin_term_def, iSUM_def]>>
+  intLib.ARITH_TAC
+QED
+
+Theorem eval_lin_term_ge_1:
+  eval_lin_term wb (MAP (λe. (1, f e)) ls) ≥ 1 ⇔
+  ∃e. MEM e ls ∧ lit wb (f e)
+Proof
+  rw[eval_lin_term_def]>>
+  Induct_on ‘ls’>>
+  rw[iSUM_def,b2i_alt]
+  >-(
+    simp[SF DNF_ss]>>
+    qmatch_goalsub_abbrev_tac`_ + iSUM lss ≥ _`>>
+    `iSUM lss ≥ 0` by (
+      irule iSUM_ge_0>>
+      simp[Abbr`lss`,MEM_MAP,PULL_EXISTS,b2i_alt]>>
+      rw[])>>
+    intLib.ARITH_TAC)
+  >- metis_tac[]
+QED
+
+(* Encodes that all As ≥ M *)
+Definition encode_Gem_ge_def:
+  encode_Gem_ge bnd As M =
+  MAP (λA. bits_imply bnd [Pos (Gem A M)] (mk_constraint_ge 1 A (-1) M 0)) As
+End
+
+(* iff versions *)
+Definition encode_Gem_ge_iff_def:
+  encode_Gem_ge_iff bnd As M =
+  encode_Gem_ge bnd As M ++
+  MAP (λA. bits_imply bnd [Neg (Gem A M)] (mk_constraint_ge 1 M (-1) A 1)) As
+End
+
+(* Encodes that all As ≤ M *)
+Definition encode_Gem_le_def:
+  encode_Gem_le bnd As M =
+  MAP (λA. bits_imply bnd [Pos (Gem M A)] (mk_constraint_ge 1 M (-1) A 0)) As
+End
+
+Definition encode_Gem_le_iff_def:
+  encode_Gem_le_iff bnd As M =
+  encode_Gem_le bnd As M ++
+  MAP (λA. bits_imply bnd [Neg (Gem M A)] (mk_constraint_ge 1 A (-1) M 1)) As
+End
+
+Theorem encode_Gem_ge_sem:
+  valid_assignment bnd wi ⇒
+  EVERY (λx. iconstraint_sem x (wi,wb)) (encode_Gem_ge bnd As M) =
+    (∀A. MEM A As ∧ wb (Gem A M) ⇒ varc wi A ≥ varc wi M)
+Proof
+  rw[encode_Gem_ge_def]>>
+  simp[EVERY_MAP,EVERY_MEM,bits_imply_sem,mk_constraint_ge_sem,GSYM integerTheory.INT_POLY_CONV_rth,integerTheory.INT_GE, integerTheory.INT_SUB_LE]>>
+  metis_tac[]
+QED
+
+Theorem encode_Gem_le_sem:
+  valid_assignment bnd wi ⇒
+  EVERY (λx. iconstraint_sem x (wi,wb)) (encode_Gem_le bnd As M) =
+    (∀A. MEM A As ∧ wb (Gem M A) ⇒ varc wi A ≤ varc wi M)
+Proof
+  rw[encode_Gem_le_def]>>
+  simp[EVERY_MAP,EVERY_MEM,bits_imply_sem,mk_constraint_ge_sem,GSYM integerTheory.INT_POLY_CONV_rth,integerTheory.INT_GE, integerTheory.INT_SUB_LE]>>
+  metis_tac[]
+QED
+
+Theorem encode_Gem_ge_iff_sem:
+  valid_assignment bnd wi ⇒
+  EVERY (λx. iconstraint_sem x (wi,wb)) (encode_Gem_ge_iff bnd As M) =
+    (∀A. MEM A As ⇒ (wb (Gem A M) ⇔ varc wi A ≥ varc wi M))
+Proof
+  rw[encode_Gem_ge_iff_def,encode_Gem_ge_sem]>>
+  simp[EVERY_MAP,EVERY_MEM,bits_imply_sem,mk_constraint_ge_sem,
+    intLib.ARITH_PROVE ``X + -1 * (Y:int) ≥ 1 ⇔ ¬ (Y ≥ X)``]>>
+  metis_tac[]
+QED
+
+Theorem encode_Gem_le_iff_sem:
+  valid_assignment bnd wi ⇒
+  EVERY (λx. iconstraint_sem x (wi,wb)) (encode_Gem_le_iff bnd As M) =
+    (∀A. MEM A As ⇒ (wb (Gem M A) ⇔ varc wi A ≤ varc wi M))
+Proof
+  rw[encode_Gem_le_iff_def,encode_Gem_le_sem]>>
+  simp[EVERY_MAP,EVERY_MEM,bits_imply_sem,mk_constraint_ge_sem,
+    intLib.ARITH_PROVE ``X + -1 * (Y:int) ≥ 1 ⇔ ¬ (X <= Y)``]>>
+  metis_tac[]
+QED
+
+Definition encode_arr_max_def:
+  encode_arr_max bnd M As =
+  ([], MAP (λA. (1, Pos (Gem A M))) As, 1) ::
+  encode_Gem_ge bnd As M ++
+  MAP (λA. mk_constraint_ge 1 M (-1) A 0) As
+End
+
+Theorem encode_arr_max_sem:
+  valid_assignment bnd wi ⇒
+  EVERY (λx. iconstraint_sem x (wi,wb)) (encode_arr_max bnd M As) = (
+    (∃A. MEM A As ∧ wb (Gem A M)) ∧
+    (∀A. MEM A As ∧ wb (Gem A M) ⇒ varc wi A ≥ varc wi M) ∧
+    arr_max_sem M As wi)
+Proof
+  strip_tac>>
+  simp[encode_arr_max_def,encode_Gem_ge_sem]>>
+  match_mp_tac LEFT_AND_CONG>>
+  CONJ_TAC >-
+    simp[iconstraint_sem_def,eval_ilin_term_def,iSUM_def,eval_lin_term_ge_1]>>
+  strip_tac>>
+  match_mp_tac LEFT_AND_CONG>> simp[]>>
+  strip_tac>>
+  simp[arr_max_sem_def,EVERY_MAP,mk_constraint_ge_sem,GSYM integerTheory.INT_POLY_CONV_rth,
+       integerTheory.INT_GE,integerTheory.INT_SUB_LE,MEM_MAP,EVERY_MEM]>>
+  iff_tac>>
+  rw[]>>
+  pop_assum drule>>
+  pop_assum drule>>
+  rw[integerTheory.INT_GE,GSYM integerTheory.INT_LE_ANTISYM]>>
+  simp[SF SFY_ss]
+QED
+
+Definition encode_arr_min_def:
+  encode_arr_min bnd M As =
+  ([], MAP (λA. (1, Pos (Gem M A))) As, 1) ::
+  encode_Gem_le bnd As M ++
+  MAP (λA. mk_constraint_ge 1 A (-1) M 0) As
+End
+
+Theorem encode_arr_min_sem:
+  valid_assignment bnd wi ⇒
+  EVERY (λx. iconstraint_sem x (wi,wb)) (encode_arr_min bnd M As) = (
+    (∃A. MEM A As ∧ wb (Gem M A)) ∧
+    (∀A. MEM A As ∧ wb (Gem M A) ⇒ varc wi A ≤ varc wi M) ∧
+    arr_min_sem M As wi)
+Proof
+  strip_tac>>
+  simp[encode_arr_min_def,encode_Gem_le_sem]>>
+  match_mp_tac LEFT_AND_CONG>>
+  CONJ_TAC >-
+    simp[iconstraint_sem_def,eval_ilin_term_def,iSUM_def,eval_lin_term_ge_1]>>
+  strip_tac>>
+  match_mp_tac LEFT_AND_CONG>> simp[]>>
+  strip_tac>>
+  simp[arr_min_sem_def,EVERY_MAP,mk_constraint_ge_sem,GSYM integerTheory.INT_POLY_CONV_rth,
+       integerTheory.INT_GE,integerTheory.INT_SUB_LE,MEM_MAP,EVERY_MEM]>>
+  iff_tac>>
+  rw[]>>
+  pop_assum drule>>
+  pop_assum drule>>
+  rw[integerTheory.INT_GE,GSYM integerTheory.INT_LE_ANTISYM]>>
+  simp[SF SFY_ss]
+QED
+
+Definition encode_count_def:
+  encode_count bnd Y C As =
+  let
+    ilpc =
+    case C of
+      INL vC => [
+        ([(-1, vC)], MAP (λA. (1, Pos (Eqc A Y))) As, 0);
+        ([(1, vC)], MAP (λA. (-1, Pos (Eqc A Y))) As, 0)]
+    | INR cC => [
+        ([], MAP (λA. (1, Pos (Eqc A Y))) As, cC);
+        ([], MAP (λA. (-1, Pos (Eqc A Y))) As, -cC)]
+  in
+    encode_Gem_ge_iff bnd As Y ++
+    encode_Gem_le_iff bnd As Y ++
+    MAP (λA. bits_imply bnd [Pos (Eqc A Y)]
+                        ([], [(1, Pos (Gem A Y)); (1, Pos (Gem Y A))], 2)) As ++
+    MAP (λA. bits_imply bnd [Neg (Eqc A Y)]
+                        ([], [(1, Neg (Gem A Y)); (1, Neg (Gem Y A))], 1)) As ++
+    ilpc
+End
+
+Theorem iSUM_MAP_lin:
+  ∀ls a f b. iSUM (MAP (λx. a * f x + b) ls) = a * iSUM (MAP (λx. f x) ls) + b * &LENGTH ls
+Proof
+  Induct>>
+  simp[iSUM_def,MAP,LENGTH]>>
+  rw[]>>
+  intLib.ARITH_TAC
+QED
+
+Theorem iSUM_MAP_lin_const = iSUM_MAP_lin |> CONV_RULE (RESORT_FORALL_CONV List.rev) |> Q.SPEC `0` |> SRULE [] |> SPEC_ALL;
+
+Theorem b2i_ge_2[simp]:
+  b2i b1 + b2i b2 ≥ 2 ⇔ b1 ∧ b2
+Proof
+  rw[b2i_alt]
+QED
+
+Theorem b2i_ge_1[simp]:
+  b2i b1 + b2i b2 ≥ 1 ⇔ b1 ∨ b2
+Proof
+  rw[b2i_alt]
+QED
+
+Theorem encode_count_sem:
+  valid_assignment bnd wi ⇒
+  EVERY (λx. iconstraint_sem x (wi,wb)) (encode_count bnd Y C As) = (
+    EVERY (λA. wb (Gem A Y) ⇔ varc wi A ≥ varc wi Y) As ∧
+    EVERY (λA. wb (Gem Y A) ⇔ varc wi Y ≥ varc wi A) As ∧
+    EVERY (λA. wb (Eqc A Y) ⇔ varc wi A = varc wi Y) As ∧
+    count_sem Y C As wi)
+Proof
+  strip_tac>>
+  simp[encode_count_def]>>
+  simp[GSYM CONJ_ASSOC]>>
+  ho_match_mp_tac LEFT_AND_CONG>>
+  CONJ_TAC >-
+    simp[encode_Gem_ge_iff_sem,EVERY_MEM]>>
+  strip_tac>>
+  ho_match_mp_tac LEFT_AND_CONG>>
+  CONJ_TAC >-
+    simp[encode_Gem_le_iff_sem,EVERY_MEM,integerTheory.INT_GE]>>
+  strip_tac>>
+  simp[CONJ_ASSOC]>>
+  ho_match_mp_tac LEFT_AND_CONG>>
+  CONJ_TAC >- (
+    fs[EVERY_MEM,MEM_MAP,PULL_EXISTS,bits_imply_sem,iconstraint_sem_def,eval_ilin_term_def,eval_lin_term_def,iSUM_def]>>
+    metis_tac[integerTheory.INT_LE_ANTISYM,integerTheory.INT_GE])>>
+  strip_tac
+  >- (
+    Cases_on ‘C’>>
+    simp[count_sem_def]>>
+    rw[METIS_PROVE[] “∀P a b. (∀x. x = a ∨ x = b ⇒ P x) ⇔ P a ∧ P b”]>>
+    simp[iconstraint_sem_def,eval_ilin_term_def,eval_lin_term_def,
+      MAP_MAP_o,combinTheory.o_ABS_R,b2i_alt,iSUM_def,Once varc_def]>>
+    ‘iSUM (MAP (λA. if wb (Eqc A Y) then 1 else 0) As) =
+     iSUM (MAP (λA. if varc wi A = varc wi Y then 1 else 0) As)’ by
+      fs[EVERY_MEM,Cong MAP_CONG]>>
+    simp[iSUM_MAP_lin_const]>>
+    intLib.ARITH_TAC)
+QED
+
+(* domain of X given by bnd *)
+Definition dom_def:
+  dom bnd X =
+  case X of
+    INL vX =>
+      let
+        (lb, ub) = bnd vX
+      in
+        if lb > ub then [] else GENLIST (λn. &n + lb) (Num (ub - lb) + 1)
+  | INR cX => [cX]
+End
+
+Definition encode_nvalue_def:
+  encode_nvalue bnd Y As =
+  let
+    Vals = nub $ FLAT $ MAP (dom bnd) As;
+    some_eq = λv. ([], MAP (λA. (1i, Pos (Eqc A (INR v)))) As, 1i);
+    none_eq = λv. ([], MAP (λA. (-1i, Pos (Eqc A (INR v)))) As, 0i)
+  in
+    MAP (λv. bits_imply bnd [Pos (Nv As v)] (some_eq v)) Vals ++
+    MAP (λv. bits_imply bnd [Neg (Nv As v)] (none_eq v)) Vals ++
+    (case Y of
+        INL vY =>
+          [([(-1, vY)], MAP (λv. (1i, Pos (Nv As v))) Vals, 0);
+          ([(1, vY)], MAP (λv. (-1i, Pos (Nv As v))) Vals, 0)]
+      | INR cY =>
+          [([], MAP (λv. (1i, Pos (Nv As v))) Vals, cY);
+          ([], MAP (λv. (-1i, Pos (Nv As v))) Vals, -cY)])
+End
+
+(* TODO: Theorem encode_nvalue_sem *)
+
+Definition encode_table_def:
+  encode_table bnd Xs Tss =
+  let n = LENGTH Xs in
+    if EVERY (λTs. LENGTH Ts = n) Tss
+    then
+      let
+        all_eq = λTs. ([], MAP (λ(X, T). (1i, Pos (Eqc X T))) (ZIP (Xs, Ts)), &n);
+        some_neq = λTs. ([], MAP (λ(X, T). (-1i, Pos (Eqc X T))) (ZIP (Xs, Ts)), -&n + 1i)
+      in
+        MAP (λTs. bits_imply bnd [Pos (Tb Xs Ts &n)] (all_eq Ts)) Tss ++
+        MAP (λTs. bits_imply bnd [Neg (Tb Xs Ts &n)] (some_neq Ts)) Tss ++
+        [([], MAP (λTs. (1i, Pos (Tb Xs Ts &n))) Tss, 1i)]
+    else [([], [], 1i)]
+End
+
+(* TODO: Theorem encode_table_sem *)
+
+(* The top-level encodings *)
+Definition encode_cp_one_def:
+  encode_cp_one bnd c =
+  case c of
+    NotEquals X Y => encode_not_equals bnd X Y
+  | AllDifferent As => encode_all_different bnd As
+  | Element R X As => encode_element bnd R X As
+  | Abs X Y => encode_abs bnd X Y
+  | Ilc Xs op rhs => encode_ilc Xs op rhs
+End
+
+Theorem encode_cp_one_sem_1:
+  valid_assignment bnd wi ∧
+  constraint_sem c wi ⇒
+  EVERY (λx. iconstraint_sem x (wi,reify_reif wi)) (encode_cp_one bnd c)
+Proof
+  Cases_on`c`>>
+  rw[encode_cp_one_def,constraint_sem_def]
+  >- (
+    simp[encode_not_equals_sem,reify_reif_def]>>
+    gvs[not_equals_sem_def]>>
+    intLib.ARITH_TAC)
+  >- (
+    simp[encode_all_different_sem,reify_reif_def]>>
+    gvs[all_different_sem_def,EL_ALL_DISTINCT_EL_EQ]>>
+    rw[]>>
+    first_x_assum(qspecl_then[`i`,`j`] mp_tac)>>
+    simp[EL_MAP]>>
+    intLib.ARITH_TAC)
+  >- (
+    simp[encode_element_sem,reify_reif_def]>>
+    every_case_tac>>simp[])
+  >- (
+    simp[encode_abs_sem,reify_reif_def]>>
+    every_case_tac>>simp[])
+  >- (
+    simp[encode_ilc_sem,reify_reif_def]>>
+    every_case_tac>>simp[])
+QED
+
+Theorem encode_cp_one_sem_2:
+  valid_assignment bnd wi ∧
+  EVERY (λx. iconstraint_sem x (wi,wb)) (encode_cp_one bnd c) ⇒
+  constraint_sem c wi
+Proof
+  Cases_on`c`>>
+  rw[encode_cp_one_def,constraint_sem_def]
+  >-
+    gvs[encode_not_equals_sem]
+  >-
+    gvs[encode_all_different_sem]
+  >-
+    gvs[encode_element_sem]
+  >-
+    gvs[encode_abs_sem]
+  >-
+    gvs[encode_ilc_sem]
+QED
+
+(* An actual implementation will avoid duplicates here *)
+Definition encode_cp_all_def:
+  encode_cp_all bnd cs =
+  FLAT (MAP (encode_cp_one bnd) cs)
+End
+
+Theorem encode_cp_all_sem_1:
+  valid_assignment bnd wi ∧
+  EVERY (λc. constraint_sem c wi) cs ⇒
+  EVERY (λx. iconstraint_sem x (wi,reify_reif wi)) (encode_cp_all bnd cs)
+Proof
+  simp[encode_cp_all_def,EVERY_FLAT]>>
+  simp[Once EVERY_MEM]>>
+  rw[Once EVERY_MEM,MEM_MAP]>>
+  metis_tac[encode_cp_one_sem_1]
+QED
+
+Theorem encode_cp_all_sem_2:
+  valid_assignment bnd wi ∧
+  EVERY (λx. iconstraint_sem x (wi,wb)) (encode_cp_all bnd cs) ⇒
+  EVERY (λc. constraint_sem c wi) cs
+Proof
+  simp[encode_cp_all_def,EVERY_FLAT]>>
+  rw[Once EVERY_MEM,MEM_MAP,PULL_EXISTS]>>
+  simp[Once EVERY_MEM]>>
+  metis_tac[encode_cp_one_sem_2]
+QED
+
+(* === Examples ===
+
+not-equals
+  EVAL``encode_not_equals (λX. (-10,10)) (INL X) (INL Y)``
+  EVAL``encode_not_equals (λX. (-10,10)) (INL X) (INR 4)``
+
+all-different
+  EVAL``encode_all_different (λX. (-10,10)) [INL X; INL Y; INL Z; INR 0i]``
+
+element
+  EVAL``encode_element (λX. (-10,10)) (INL R) (INL X) [INL A; INL B; INL C; INL D; INL E]``
+
+abs
+  EVAL``encode_abs (λX. (-10,10)) (INL X) (INL Y)``
+
+*)
+
+val _ = export_theory();
